full correctness for serialization that skips data

systems/Serialized.v
@@ -6,7 +6,6 @@ Set Implicit Arguments.
 Section Serialized.
   Context {orig_base_params : BaseParams}.
   Context {orig_multi_params : MultiParams orig_base_params}.
-  Context {orig_data_serializer : Serializer data}.
   Context {orig_input_serializer : Serializer input}.
   Context {orig_output_serializer : Serializer output}.
   Context {orig_msg_serializer : Serializer msg}.
@@ -16,50 +15,38 @@ Section Serialized.
     (n, serialize msg).
 
   Definition serialize_handler_result (result : (list output) * data * list (name * msg)) :
-    list (list bool) * list bool * list (name * list bool) :=
+    list (list bool) * data * list (name * list bool) :=
     let '(outputs, data, messages) := result in
     let outputsBits := map (@serialize output orig_output_serializer) outputs in
-    let dataBits := serialize data in
     let messagesBits := map serialize_name_msg_tuple messages in
-    (outputsBits, dataBits, messagesBits).
-
-  Definition serialized_init_handlers (n : name) :=
-    serialize (init_handlers n).
+    (outputsBits, data, messagesBits).
 
   Definition serialized_net_handlers
              (dst : name)
              (src : name)
              (mBits : list bool)
-             (stateBits : list bool) :
-    list (list bool) * list bool * list (name * list bool) :=
+             (d : data) :
+    list (list bool) * data * list (name * list bool) :=
     match (deserialize mBits) with
-    | None => ([], stateBits, [])
+    | None => ([], d, [])
     | Some (m, rest) =>
-      match (deserialize stateBits) with
-      | None => ([], stateBits, [])
-      | Some (state, rest) =>
-        serialize_handler_result (net_handlers dst src m state)
-      end
+      serialize_handler_result (net_handlers dst src m d)
     end.
 
   Definition serialized_input_handlers
              (h : name)
              (inpBits : list bool)
-             (stateBits : list bool) :
-    list (list bool) * list bool * list (name * list bool) :=
+             (d : data) :
+    list (list bool) * data * list (name * list bool) :=
     match (deserialize inpBits) with
-    | None => ([], stateBits, [])
+    | None => ([], d, [])
     | Some (inp, rest) =>
-      match (deserialize stateBits) with
-      | None => ([], stateBits, [])
-      | Some (state, rest) =>
-        serialize_handler_result (input_handlers h inp state)
-      end
+      serialize_handler_result (input_handlers h inp d)
     end.
 
   Instance base_params : BaseParams :=
     {
-      data := list bool;
+      data := data;
       input := list bool;
       output := list bool
     }.
@@ -71,7 +58,7 @@ Section Serialized.
       msg := list bool;
       msg_eq_dec := (list_eq_dec Bool.bool_dec);
       nodes := nodes;
-      init_handlers := serialized_init_handlers;
+      init_handlers := init_handlers;
       net_handlers := serialized_net_handlers;
       input_handlers := serialized_input_handlers;
     }.
